{
 "cells": [
  {
   "cell_type": "markdown",
   "id": "11daf07f",
   "metadata": {},
   "source": [
    "(co-ordinate-geometry-exercises-section)=\n",
    "# Co-ordinate geometry exercises\n",
    "\n",
    "::::{admonition} Exercise 4.1\n",
    "The points $A, B, C, D$ in $\\mathbb{R}^3$ have the following position vectors\n",
    "\n",
    "\\begin{align*}\n",
    "    \\mathbf{a} &= \\begin{pmatrix} 2 \\\\ 1 \\\\ 0 \\end{pmatrix}, &\n",
    "    \\mathbf{b} &= \\begin{pmatrix} 1 \\\\ 1 \\\\ 0 \\end{pmatrix}, &\n",
    "    \\mathbf{c} &= \\begin{pmatrix} 3 \\\\ -1 \\\\ 4 \\end{pmatrix}, &\n",
    "    \\mathbf{d} &= \\begin{pmatrix} 5 \\\\ 2 \\\\ 6 \\end{pmatrix}.\n",
    "\\end{align*}\n",
    "\n",
    "Find:\n",
    "\n",
    "(a) &emsp; the equation of the line that passes through $A$ and $B$;\n",
    "\n",
    ":::{dropdown} Solution\n",
    "\n",
    "Using the [vector equation of a line](vector-equation-of-a-line-definition) then $Q = \\mathbf{a} + t\\mathbf{d}_1$\n",
    "\n",
    "\\begin{align*}\n",
    "    \\mathbf{d}_1 &= \\mathbf{b} - \\mathbf{a} =\n",
    "    \\begin{pmatrix} 1 \\\\ 1 \\\\ 0 \\end{pmatrix} -\n",
    "    \\begin{pmatrix} 2 \\\\ 1 \\\\ 0 \\end{pmatrix} = \n",
    "    \\begin{pmatrix} -1 \\\\ 0 \\\\ 0 \\end{pmatrix}, \\\\\n",
    "    \\therefore Q &= \\mathbf{a} + t\\mathbf{d}_1 =\n",
    "    \\begin{pmatrix} 2 \\\\ 1 \\\\ 0 \\end{pmatrix} + t \n",
    "    \\begin{pmatrix} -1 \\\\ 0 \\\\ 0 \\end{pmatrix} = \n",
    "    \\begin{pmatrix} 2 - t \\\\ 1 \\\\ 1 \\end{pmatrix}\n",
    "\\end{align*}\n",
    ":::\n",
    "\n",
    "(b) &emsp; the equation of the line that passes through $C$ and $D$;\n",
    "\n",
    ":::{dropdown} Solution\n",
    "\n",
    "Using the [vector equation of a line](vector-equation-of-a-line-definition) then $Q = \\mathbf{c} + t\\mathbf{d}_2$\n",
    "\n",
    "\\begin{align*}\n",
    "    \\mathbf{d}_2 &= \\mathbf{d} - \\mathbf{c} =\n",
    "    \\begin{pmatrix} 5 \\\\ 2 \\\\ 6 \\end{pmatrix} -\n",
    "    \\begin{pmatrix} 3 \\\\ -1 \\\\ 4 \\end{pmatrix} = \n",
    "    \\begin{pmatrix} 2 \\\\ 3 \\\\ 2 \\end{pmatrix}, \\\\\n",
    "    \\therefore Q &= \\mathbf{c} + t\\mathbf{d}_2 =\n",
    "    \\begin{pmatrix} 3 \\\\ -1 \\\\ 4 \\end{pmatrix} + t \n",
    "    \\begin{pmatrix} 2 \\\\ 3 \\\\ 2 \\end{pmatrix} = \n",
    "    \\begin{pmatrix} 3 + 2 t \\\\ -1 + 3 t \\\\ 4 + 2 t \\end{pmatrix}\n",
    "\\end{align*}\n",
    ":::\n",
    "\n",
    "(c) &emsp; the equation of the plane which $A$, $B$ and $C$ lie on;\n",
    "\n",
    ":::{dropdown} Solution\n",
    "\\begin{align*}\n",
    "    \\overrightarrow{AB} &= \\begin{pmatrix} 1 \\\\ 1 \\\\ 0 \\end{pmatrix} - \n",
    "    \\begin{pmatrix} 2 \\\\ 1 \\\\ 0 \\end{pmatrix} = \n",
    "    \\begin{pmatrix} -1 \\\\ 0 \\\\ 0 \\end{pmatrix}, \\\\\n",
    "    \\overrightarrow{AC} &= \\begin{pmatrix} 3 \\\\ -1 \\\\ 4 \\end{pmatrix} -\n",
    "    \\begin{pmatrix} 2 \\\\ 1 \\\\ 0 \\end{pmatrix} =\n",
    "    \\begin{pmatrix} 1 \\\\ -2 \\\\ 4 \\end{pmatrix}, \\\\\n",
    "    \\therefore \\mathbf{n} &= \\overrightarrow{AB} \\times \\overrightarrow{AC} = \n",
    "    \\begin{vmatrix} \n",
    "        \\mathbf{i} & \\mathbf{j} & \\mathbf{k} \\\\\n",
    "        -1 & 0 & 0 \\\\\n",
    "        1 & -2 & 4 \n",
    "    \\end{vmatrix} =\n",
    "    \\begin{pmatrix} 0 \\\\ 4 \\\\ 2 \\end{pmatrix},\n",
    "\\end{align*}\n",
    "\n",
    "Using the [point normal definition of a plane](point-normal-definition)\n",
    "\\begin{align*}\n",
    "    \\mathbf{n} \\cdot \\begin{pmatrix} x - x_0 \\\\ y - y_0 \\\\ z - z_0 \\end{pmatrix} &= 0 \\\\\n",
    "    \\begin{pmatrix} 0 \\\\ 4 \\\\ 2 \\end{pmatrix} \\cdot \\begin{pmatrix} x - 1 \\\\ y - 1 \\\\ z - 0 \\end{pmatrix} &= 0 \\\\\n",
    "    4 y + 2 z - 4 &= 0.\n",
    "\\end{align*}\n",
    ":::\n",
    "\n",
    "\n",
    "(d) &emsp; the equation of the plane which $B$, $C$ and $D$ lie on.\n",
    "\n",
    ":::{dropdown} Solution\n",
    "\\begin{align*}\n",
    "    \\overrightarrow{BC} &= \\begin{pmatrix} 3 \\\\ -1 \\\\ 4 \\end{pmatrix} - \n",
    "    \\begin{pmatrix} 1 \\\\ 1 \\\\ 0 \\end{pmatrix} =\n",
    "    \\begin{pmatrix} 2 \\\\ -2 \\\\ 4 \\end{pmatrix}, \\\\\n",
    "    \\overrightarrow{BD} &= \\begin{pmatrix} 5 \\\\ 2 \\\\ 6 \\end{pmatrix} -\n",
    "    \\begin{pmatrix} 1 \\\\ 1 \\\\ 0 \\end{pmatrix} =\n",
    "    \\begin{pmatrix} 4 \\\\ 1 \\\\ 6 \\end{pmatrix}, \\\\\n",
    "    \\mathbf{n} &= \\overrightarrow{BC} \\times \\overrightarrow{BD} = \n",
    "    \\begin{vmatrix}\n",
    "        \\mathbf{i} & \\mathbf{j} & \\mathbf{k} \\\\\n",
    "        2 & -2 & 4 \\\\\n",
    "        4 & 1 & 6\n",
    "    \\end{vmatrix} =\n",
    "    \\begin{pmatrix} -16 \\\\ 4 \\\\ 10 \\end{pmatrix},\n",
    "\\end{align*}\n",
    "\n",
    "Using the [point normal definition of a plane](point-normal-definition)\n",
    "\n",
    "\\begin{align*}\n",
    "    \\mathbf{n} \\cdot \\begin{pmatrix} x - x_0 \\\\ y - y_0 \\\\ z - z_0 \\end{pmatrix} &= 0 \\\\\n",
    "    \\begin{pmatrix} -16 \\\\ 4 \\\\ 10 \\end{pmatrix} \\cdot \n",
    "    \\begin{pmatrix} x - 1 \\\\ y - 1 \\\\ z - 0 \\end{pmatrix} &= 0 \\\\\n",
    "    -16 x + 4 y + 10 z + 12 &= 0.\n",
    "\\end{align*}\n",
    ":::\n",
    "\n",
    "::::\n",
    "\n",
    "::::{admonition} Exercise 4.2\n",
    "Find the equation of the line that passes through the point $(3, 2, 1)$ which is parallel to $2 \\mathbf{i} + \\mathbf{j} + 3 \\mathbf{k}$.\n",
    "\n",
    ":::{dropdown} Solution\n",
    "$$ Q = \\begin{pmatrix} 3 \\\\ 2 \\\\ 1 \\end{pmatrix} + t \\begin{pmatrix} 2 \\\\ 3 \\\\ 1 \\end{pmatrix}  = \\begin{pmatrix} 3 + 2 t \\\\ 2 + 3 t \\\\ 1 + 3 t \\end{pmatrix} $$\n",
    ":::\n",
    "\n",
    "::::\n",
    "\n",
    "::::{admonition} Exercise 4.3\n",
    "Find the equation of the plane that passes through the point $(3, 2, 5)$ which has a normal vector $\\mathbf{n} = (2, 1, 3)$.\n",
    "\n",
    ":::{dropdown} Solution\n",
    "Using the [point normal definition of a plane](point-normal-definition)\n",
    "\\begin{align*}\n",
    "    \\mathbf{n} \\cdot \\begin{pmatrix} x - x_0 \\\\ y - y_0 \\\\ z - z_0 \\end{pmatrix} &= 0 \\\\\n",
    "    \\begin{pmatrix} 2 \\\\ 1 \\\\ 3 \\end{pmatrix} \\cdot\n",
    "    \\begin{pmatrix} x - 3 \\\\ y - 2 \\\\ z - 5 \\end{pmatrix} \\\\\n",
    "    2(x - 3) + (y - 2) + 3(z - 5) &= 0 \\\\\n",
    "    2 x + y + 3 z - 23 &= 0\n",
    "\\end{align*}\n",
    ":::\n",
    "::::\n",
    "\n",
    "::::{admonition} Exercise 4.4\n",
    "Two lines in $\\mathbb{R}^3$ are defined by $\\ell_1: (1 + 2t, -t, 1 + 3t)$ and $\\ell_2: (1 + 2t, 4, 7 - t)$ respectively.\n",
    "\n",
    "(a) &emsp; find the intersection of the lines or show they are skew;\n",
    "\n",
    ":::{dropdown} Solution\n",
    "Equating $\\ell_1$ and $\\ell_2$ and attempting to solve for $t$\n",
    "\\begin{align*}\n",
    "    1 + 2t &= 1 + 2t \\\\\n",
    "    -t &= 4 \\\\\n",
    "    1 + 3t &= 7 - t\n",
    "\\end{align*}\n",
    "\n",
    "From the second equation $t = -4$ which when substituted into the third equation gives $-11 = 11$ which is a contradiction, therefore $\\ell_1$ and $\\ell_2$ do not intersect. \n",
    "\n",
    "We also need to show that they are not parallel, i.e., there is no value $k$ such that $\\mathbf{d}_1 = k \\mathbf{d}_2$. The direction vectors for $\\ell_1$ and $\\ell_2$ are $\\mathbf{d}_1 = (2, -1, 3)$ and $\\mathbf{d}_2 = (2, 0, -1)$ so\n",
    "\n",
    "\\begin{align*}\n",
    "    \\begin{pmatrix} 2 \\\\ -1 \\\\ 3 \\end{pmatrix} &= k \\begin{pmatrix} 2 \\\\ 0 \\\\ -1 \\end{pmatrix},\n",
    "\\end{align*}\n",
    "\n",
    "which gives the system\n",
    "\n",
    "\\begin{align*}\n",
    "    2 &= 2k ,\\\\\n",
    "    -1 &= 0, \\\\\n",
    "    3 &= -k.\n",
    "\\end{align*}\n",
    "\n",
    "The second equation is a contradiction so $\\ell_1$ and $\\ell_2$ are not parallel, and since they do not intersect then they must be skew.\n",
    ":::\n",
    "\n",
    "(b) &emsp; find the shortest distance between the lines;\n",
    "\n",
    ":::{dropdown} Solution\n",
    "Here $\\ell_1$ is $P_1 + t\\mathbf{d}_1 = (1, 0, 1) + t(2, -1, 3)$ and $\\ell_2$ is $P_2 + \\mathbf{d}_2 = (1, 4, 7) + t(2, 0, -1)$, so calculating a vector perpendicular to both $\\ell_1$ and $\\ell_2$ gives\n",
    "\n",
    "\\begin{align*}\n",
    "    \\mathbf{n} &= \\mathbf{d}_1 \\times \\mathbf{d_1} = \\begin{pmatrix} 2 \\\\ -1 \\\\ 3 \\end{pmatrix} \\times\n",
    "    \\begin{pmatrix} 2 \\\\ 0 \\\\ -1 \\end{pmatrix} =\n",
    "    \\begin{vmatrix}\n",
    "        \\mathbf{i} & \\mathbf{j} & \\mathbf{k} \\\\\n",
    "        2 & -1 & 3 \\\\\n",
    "        2 & 0 & -1 \n",
    "    \\end{vmatrix} = \n",
    "    \\begin{pmatrix} 1 \\\\ 8 \\\\ 2 \\end{pmatrix}, \\\\\n",
    "\\end{align*}\n",
    "\n",
    "and normalising gives\n",
    "\n",
    "\\begin{align*}\n",
    "    \\hat{\\mathbf{n}} = \\frac{\\mathbf{n}}{|\\mathbf{n}|} = \\frac{1}{\\sqrt{69}} \n",
    "    \\begin{pmatrix} 1 \\\\ 8 \\\\ 2 \\end{pmatrix} =\n",
    "    \\begin{pmatrix} \\frac{\\sqrt{69}}{69} \\\\ \\frac{8\\sqrt{69}}{69} \\\\ \\frac{2\\sqrt{69}}{69} \\end{pmatrix}.\n",
    "\\end{align*}\n",
    "\n",
    "Using [the distance between two lines](line-line-distance-definition)\n",
    "\n",
    "\\begin{align*}\n",
    "    d &= (\\mathbf{p}_2 - \\mathbf{p}_1) \\cdot \\hat{\\mathbf{n}} \\\\\n",
    "    &= \\left( \\begin{pmatrix} 1 \\\\ 4 \\\\ 7 \\end{pmatrix} -\n",
    "    \\begin{pmatrix} 1 \\\\ 0 \\\\ 1 \\end{pmatrix} \\right) \\cdot\n",
    "    \\begin{pmatrix} \\frac{\\sqrt{69}}{69} \\\\ \\frac{8\\sqrt{69}}{69} \\\\ \\frac{2\\sqrt{69}}{69} \\end{pmatrix} \\\\\n",
    "    &= \\begin{pmatrix} 0 \\\\ 4 \\\\ 6 \\end{pmatrix} \\cdot\n",
    "    \\begin{pmatrix} \\frac{\\sqrt{69}}{69} \\\\ \\frac{8\\sqrt{69}}{69} \\\\ \\frac{2\\sqrt{69}}{69} \\end{pmatrix} \\\\\n",
    "    &= \\frac{44\\sqrt{69}}{69}.\n",
    "\\end{align*}\n",
    ":::\n",
    "\n",
    "(c) &emsp; find the distance between the point $P = (0, -1, 3)$ and $\\ell_1$.\n",
    "\n",
    ":::{dropdown} Solution\n",
    "Using the [shortest distance between a point and a line](point-line-distance-definition)\n",
    "\n",
    "\\begin{align*}\n",
    "    t &= \\frac{(P - P_1)\\cdot \\mathbf{d}_1}{\\mathbf{d}_1 \\cdot \\mathbf{d}_1} = \\frac{ \n",
    "    \\left( \\begin{pmatrix} 0 \\\\ -1 \\\\ 3 \\end{pmatrix} -\n",
    "    \\begin{pmatrix} 1 \\\\ 0 \\\\ 1 \\end{pmatrix} \\right) \\cdot\n",
    "    \\begin{pmatrix} 2 \\\\ -1 \\\\ 3 \\end{pmatrix}}{\n",
    "        \\begin{pmatrix} 2 \\\\ -1 \\\\ 3 \\end{pmatrix} \\cdot\n",
    "        \\begin{pmatrix} 2 \\\\ -1 \\\\ 3 \\end{pmatrix}\n",
    "    } \n",
    "    = \\frac{5}{14}, \\\\\n",
    "    \\therefore Q &= P_1 + t\\mathbf{d}_1 = \\begin{pmatrix} 1 \\\\ 0 \\\\ 1 \\end{pmatrix} + \\frac{5}{14} \n",
    "    \\begin{pmatrix} 2 \\\\ -1 \\\\ 3 \\end{pmatrix} = \n",
    "    \\begin{pmatrix} \\frac{12}{7} \\\\ - \\frac{5}{14} \\\\ \\frac{29}{14} \\end{pmatrix}, \\\\\n",
    "    \\overrightarrow{QP} &= \\begin{pmatrix} 0 \\\\ -1 \\\\ 3 \\end{pmatrix} - \n",
    "    \\begin{pmatrix} \\frac{12}{7} \\\\ -\\frac{5}{14} \\\\ \\frac{29}{14} \\end{pmatrix} =\n",
    "    \\begin{pmatrix} -\\frac{12}{7} \\\\ -\\frac{9}{14} \\\\ \\frac{13}{14} \\end{pmatrix}, \\\\\n",
    "    \\therefore |\\overrightarrow{QP}| &= \n",
    "    \\sqrt{\\left(-\\frac{12}{7}\\right)^2 + \\left(-\\frac{9}{14}\\right)^2 + \\left(\\frac{13}{14}\\right)^2} \n",
    "    = \\frac{\\sqrt{826}}{14}.\n",
    "\\end{align*}\n",
    ":::\n",
    "::::\n",
    "\n",
    "::::{admonition} Exercise 4.5\n",
    "A plane has the equation $3x - 2y + z = 10$. Identify the normal to the plane and find the co-ordinates of 2 points on the plane having $z = 2$.\n",
    "\n",
    ":::{dropdown} Solution\n",
    "$\\mathbf{n} = (3, -2, 1)$. \n",
    "\n",
    "Let $x=0$ then $3(0) - 2 y + 2 = 10$ so $y = -4$ and a point on the plane has co-ordinates $(0, -4, 2)$.\n",
    "\n",
    "Let $x = 2$ then $3(2) - 2 y + 2 = 10$ so $y = -1$ and a point on the plane has co-ordinates $(2, -4, -1)$.\n",
    ":::\n",
    "::::\n",
    "\n",
    "::::{admonition} Exercise 4.6\n",
    "Find the point where the line $Q = (1 + 2t, 2 + t, -1 + 4t)$ meets the plane $6x - y - 4z = 3$. \n",
    "\n",
    ":::{dropdown} Solution\n",
    "\n",
    "First we need to find the co-ordinates of a point, $R$ say, that lies on the plane. Let $x=0$ and $y=1$ then $z=-1$ so we know that $R = (0, 1, -1)$ lies on the plane. Using the [point normal definition of a plane](point-normal-definition)\n",
    "\n",
    "\\begin{align*}\n",
    "    \\mathbf{n} \\cdot \\begin{pmatrix} x - x_0 \\\\ y - y_0 \\\\ z - z_0 \\end{pmatrix} &= 0 \\\\\n",
    "    \\begin{pmatrix} 6 \\\\ -1 \\\\ -4 \\end{pmatrix} \\cdot\n",
    "    \\begin{pmatrix} 0 - (1 + 2 t) \\\\ 1 - (2 + t) \\\\ -1 - (-1 + 4 t) \\end{pmatrix} &= 0 \\\\\n",
    "    \\begin{pmatrix} 6 \\\\ -1 \\\\ -4 \\end{pmatrix} \\cdot\n",
    "    \\begin{pmatrix} - 1 - 2 t \\\\ -1 - t \\\\  -4 t \\end{pmatrix} &= 0 \\\\\n",
    "    -6 - 12 t + 1 + t + 16 t &= 0 \\\\\n",
    "    5 t - 5 &= 0 \\\\\n",
    "    \\therefore t = 1.\n",
    "\\end{align*}\n",
    "\n",
    "So the line intersects with the plane at\n",
    "\n",
    "\\begin{align*}\n",
    "    P + t \\mathbf{d} = \n",
    "    \\begin{pmatrix} 1 \\\\ 2 \\\\ -1 \\end{pmatrix} + \n",
    "    \\begin{pmatrix} 2 \\\\ 1 \\\\ 4 \\end{pmatrix} =\n",
    "    \\begin{pmatrix} 3 \\\\ 3 \\\\ 3 \\end{pmatrix}.\n",
    "\\end{align*}\n",
    ":::\n",
    "::::\n",
    "\n",
    "::::{admonition} Exercise 4.7\n",
    ":class: note\n",
    ":name: ex4.7\n",
    "Consider the diagram below that shows a plane that passes through the point $\\mathbf{p}$ and has normal vector $\\mathbf{n}$ and the point with position $\\mathbf{q}$ not on the plane. \n",
    "\n",
    ":::{figure} ../Images/point_plane_distance.png\n",
    ":::\n",
    "\n",
    "Using the [geometric definition of a dot product](dot-product-definition) derive an expression for calculating the shortest distance between a point and a plane. Use your expression to find the shortest distance from the point $(2, 4, -3)$ to the plane $6x - y - 4z = 3$.\n",
    "\n",
    ":::{dropdown} Solution\n",
    "Using the [geometric definition of a dot product](dot-product-definition)\n",
    "\n",
    "\\begin{align*}\n",
    "    (Q - P)\\cdot \\mathbf{n} &= |\\mathbf{n}||Q - P| \\cos(\\theta).\n",
    "\\end{align*}\n",
    "\n",
    "Since $d$ is the length of the adjacent side of the right-angled triangle then\n",
    "\n",
    "\\begin{align*}\n",
    "    \\cos(\\theta) &= \\frac{d}{|Q - P|},\n",
    "\\end{align*}\n",
    "\n",
    "So\n",
    "\n",
    "\\begin{align*}\n",
    "    (Q - P) \\cdot \\mathbf{n} &= |\\mathbf{n}| |Q - P| \\frac{d}{|Q - P|} \\\\\n",
    "    \\therefore d &= (Q - P)\\cdot \\frac{\\mathbf{n}}{|\\mathbf{n}|}.\n",
    "\\end{align*}\n",
    "\n",
    "The equation of the plane is $6 x-y-4 z=3$ so letting $x=0$ and $y=1$ then $z = 1$ so we know that $P = (0, 1, -1)$ lies on the plane. Since $Q = (2, 4, -3)$ and $\\mathbf{n} = (6, -1, -4)$ then applying the above formula gives\n",
    "\n",
    "\\begin{align*}\n",
    "    d &= \\left( \\begin{pmatrix} 2 \\\\ 4 \\\\ -3 \\end{pmatrix} -\n",
    "    \\begin{pmatrix} 0 \\\\ 1 \\\\ -1 \\end{pmatrix} \\right) \\cdot \n",
    "    \\begin{pmatrix} 6 \\\\ -1 \\\\ -4 \\end{pmatrix} / \\left|\n",
    "    \\begin{pmatrix} 6 \\\\ -1 \\\\ -4 \\end{pmatrix} \\right| \\\\\n",
    "    &= \\begin{pmatrix} 2 \\\\ 3 \\\\ -2 \\end{pmatrix} \\cdot \\frac{1}{\\sqrt{53}} \n",
    "    \\begin{pmatrix} 6 \\\\ -1 \\\\ -4 \\end{pmatrix} \\\\\n",
    "    &= \\frac{12 - 3 + 8}{\\sqrt{53}} = \\frac{17}{\\sqrt{53}}\n",
    "\\end{align*}\n",
    ":::\n",
    "::::"
   ]
  }
 ],
 "metadata": {
  "kernelspec": {
   "display_name": "Python 3",
   "language": "python",
   "name": "python3"
  },
  "language_info": {
   "codemirror_mode": {
    "name": "ipython",
    "version": 3
   },
   "file_extension": ".py",
   "mimetype": "text/x-python",
   "name": "python",
   "nbconvert_exporter": "python",
   "pygments_lexer": "ipython3",
   "version": "3.8.3"
  }
 },
 "nbformat": 4,
 "nbformat_minor": 5
}